Refactor to allow customizing the state type

src/arch/x64/X64.Machine_s.fst
@@ -1,38 +1,10 @@
 module X64.Machine_s
 
-open FStar.BaseTypes
-open FStar.Map
-
-module M = TransparentMap
-
-(* Define some transparently refined int types,
-   since we only use them in specs, not in emitted code *)
 unfold let nat32_max = 0x100000000
 unfold let nat64_max = 0x10000000000000000
-let _ = assert_norm (pow2 32 = nat32_max)    (* Sanity check our constant *)
-let _ = assert_norm (pow2 64 = nat64_max)    (* Sanity check our constant *)
 type nat64 = x:nat{x < nat64_max}
-type uint64 = FStar.UInt64.t
+assume val int_to_nat64 : i:int -> n:nat64{0 <= i && i < nat64_max ==> i == n}
 
-(* map type from the F* library, it needs the key type to have decidable equality, not an issue here *)
-let map (key:eqtype) (value:Type) = FStar.Map.t key value
-
-// [@"opaque_to_smt"]
-let tmap (key:eqtype) (value:Type) = M.map key value
-// [@"opaque_to_smt"]
-let tsel = M.sel
-// [@"opaque_to_smt"]
-let tupd = M.upd 
-
-(* syntax for map accesses, m.[key] and m.[key] <- value *)
-(* as we are mostly interested in register maps in this branch, 
-   they get the fancy notation treatment*)
-unfold
-let op_String_Access     = tsel
-unfold
-let op_String_Assignment = tupd
-
-(* Define the operators we support *)
 type reg =
   | Rax
   | Rbx
@@ -51,100 +23,24 @@ type reg =
   | R14
   | R15
 
-unfold
-let reg_to_int (r : reg) : int =
-  match r with
-  | Rax -> 0
-  | Rbx -> 1
-  | Rcx -> 2
-  | Rdx -> 3
-  | Rsi -> 4
-  | Rdi -> 5
-  | Rbp -> 6
-  | Rsp -> 7
-  | R8 -> 8
-  | R9 -> 9
-  | R10 -> 10
-  | R11 -> 11
-  | R12 -> 12
-  | R13 -> 13
-  | R14 -> 14
-  | R15 -> 15
-
 type maddr =
-  | MConst : n:nat -> maddr
-  | MReg   : r:reg -> offset:int -> maddr
-  | MIndex : base:reg -> scale:int -> index:reg -> offset:int -> maddr
+  | MConst: n:int -> maddr
+  | MReg: r:reg -> offset:int -> maddr
+  | MIndex: base:reg -> scale:int -> index:reg -> offset:int -> maddr
 
 type operand =
-  | OConst: n:uint64 -> operand
-  | OReg  : r:reg -> operand
-  | OMem  : m:maddr -> operand
+  | OConst: n:int -> operand
+  | OReg: r:reg -> operand
+  | OMem: m:maddr -> operand
 
 type precode (t_ins:Type0) (t_ocmp:Type0) =
-  | Ins   : ins:t_ins -> precode t_ins t_ocmp
-  | Block : block:list (precode t_ins t_ocmp) -> precode t_ins t_ocmp
+  | Ins: ins:t_ins -> precode t_ins t_ocmp
+  | Block: block:list (precode t_ins t_ocmp) -> precode t_ins t_ocmp
   | IfElse: ifCond:t_ocmp -> ifTrue:precode t_ins t_ocmp -> ifFalse:precode t_ins t_ocmp -> precode t_ins t_ocmp
-  | While : whileCond:t_ocmp -> whileBody:precode t_ins t_ocmp -> inv:operand -> precode t_ins t_ocmp
+  | While: whileCond:t_ocmp -> whileBody:precode t_ins t_ocmp -> inv:operand -> precode t_ins t_ocmp
 
 let valid_dst (o:operand) : bool =
   not(OConst? o || (OReg? o && Rsp? (OReg?.r o)))
 
-type dst_op = o:operand { valid_dst o }
+type dst_op = o:operand{valid_dst o}
 
-(* TODO: Eventually this should be a map to bytes.  Simplifying for now *)
-type mem = map int uint64
-
-(* state type, noeq qualifier means that this type does not have decidable equality (because of the maps) *)
-noeq type state = {
-  ok  :bool;
-  regs: tmap int uint64;
-  flags:uint64;
-  mem :mem;
-}
-
-(*
- * writing all the functions as Tot functions
- *)
-unfold let eval_reg (r:reg) (s:state) :uint64 =
-  s.regs.[reg_to_int r]
-
-(*
-let valid_resolved_addr (ptr:int) (m:mem) :bool =
-  m `contains` ptr /\
-  m `contains` ptr + 1 /\
-  m `contains` ptr + 2 /\
-  m `contains` ptr + 3
-*)
-
-unfold let eval_mem (ptr:int) (s:state) :uint64 =
-  sel s.mem ptr
-
-let eval_maddr (m:maddr) (s:state) :int =
-  let open FStar.UInt64 in
-  let open FStar.Mul in
-    match m with
-    | MConst n -> n
-    | MReg reg offset -> v (eval_reg reg s) + offset
-    | MIndex base scale index offset -> v (eval_reg base s) + scale * v (eval_reg index s) + offset
-
-let eval_operand (o:operand) (s:state) :uint64 =
-  match o with
-  | OConst n -> n
-  | OReg r   -> eval_reg r s
-  | OMem m   -> eval_mem (eval_maddr m s) s
-
-let update_reg' (r:reg) (v:uint64) (s:state) :state = { s with regs = s.regs.[reg_to_int r] <- v }
-
-let update_mem (ptr:int) (v:uint64) (s:state) :state = { s with mem = upd s.mem ptr v }
-
-let valid_maddr (m:maddr) (s:state) :bool =
-  s.mem `contains` (eval_maddr m s)
-
-let valid_operand (o:operand) (s:state) :bool =
-  not (OMem? o) || (OMem? o && valid_maddr (OMem?.m o) s)
-
-(*
- * while construct has a loop invariant
- * currently it is a mem_opr, but we could introduce an expression language to enrich it
- *)
