src/arch/x64/X64.Vale.Lemmas_i.fst
@@ -1,0 +1,26 @@
+module X64.Vale.Lemmas_i
+open X64.Machine_s
+open X64.Vale.State_i
+open FStar.UInt
+module S = X64.Semantics_s
+
+#reset-options "--initial_fuel 2 --max_fuel 2"
+
+let lemma_cmp_eq s o1 o2 = ()
+let lemma_cmp_ne s o1 o2 = ()
+let lemma_cmp_le s o1 o2 = ()
+let lemma_cmp_ge s o1 o2 = ()
+let lemma_cmp_lt s o1 o2 = ()
+let lemma_cmp_gt s o1 o2 = ()
+
+let lemma_block (b0:codes) (s0:state) (sN:state) =
+  let c1::b1 = b0 in
+  let s0' = state_to_S s0 in
+  let Some s1' = S.eval_code c1 s0' in
+  let s1 = state_of_S s1' in
+  (s1, c1, b1)
+
+let lemma_empty (s0:state) (sN:state) = s0
+
+let lemma_ifElse (ifb:S.ocmp) (ct:code) (cf:code) (s0:state) (sN:state) =
+  (eval_ocmp s0 ifb, s0)
